rupicola/io/IO.fsti
@@ -10,6 +10,7 @@ module IO
 include BaseTypes
 open Hist
 open Trace
+open FStar.List.Tot
 
 val io (a:Type u#a) : Type u#a
 
@@ -27,17 +28,32 @@ val write (x:bool) : io (resexn unit)
 
 val theta : #a:Type -> io a -> hist a
 
+val io_bind_equivalence #a #b (k k':a -> io b) (m:io a) (h:history) :
+  Lemma (requires forall x. k x == k' x)
+        (ensures forall p. theta (io_bind m k) h p == theta (io_bind m k') h p)
+
 let return = io_return
 let (let!@) = io_bind
 
-val theta_history_independence #a (m:io a) (h:history) (lt:local_trace h) (fs_r:a) (p:hist_post h a) :
+val lem_theta_return #a (x:a) (h:history) (lt:local_trace h) :
+  Lemma (requires lt == [])
+        (ensures forall p. theta (return x) h p ==> p lt x)
+
+val lem_theta_bind #a #b (m:io a) (h:history) (lt2:local_trace h) (fs_r_m:a) (k:a -> io b) (lt3:local_trace (h++lt2)) (fs_r:b) (lt:local_trace h) :
+  Lemma (requires (forall (p:hist_post h a). theta m h p ==> p lt2 fs_r_m) /\
+                  (forall (p':hist_post (h++lt2) b). theta (k fs_r_m) (h++lt2) p' ==> p' lt3 fs_r) /\
+                  (lt == lt2 @ lt3))
+        (ensures forall (p_:hist_post h b). theta (io_bind m k) h p_ ==> p_ lt fs_r)
+// theta (io_bind m k) == pred transformer bind of (theta m) (fun x -> theta (k x))
+
+val theta_history_independence #a (m:io a) (h:history) (lt:local_trace h) (fs_r:a) :
   Lemma (requires forall p. theta m h p ==> p lt fs_r)
-        (ensures forall h' (lt':local_trace h') p'. theta m h' p' ==> p' lt' fs_r)
+        (ensures forall h' (lt':local_trace h') p'. theta m h' p' ==> p' lt' fs_r) // use steps e e' h lt and construct_local_trace
 
 val theta_history_independence' (#a:Type) (m:io a) (h:history) (p:hist_post h a) :
   Lemma (requires theta m h p)
         (ensures forall h'. exists (p':hist_post h' a). (theta m h' p') /\
-                 (forall (lt:local_trace h) (lt':local_trace h') r. p lt r ==> p' lt' r))
+                 (forall (lt:local_trace h) (lt':local_trace h') r. (lt == lt') ==> (p lt r <==> p' lt' r)))
 
 val post_condition_history_independence (#a:Type) (m:io a) (h h':history) (p:hist_post h a) (p':hist_post h' a) (lt':local_trace h') (r:a) :
   Lemma (requires theta m h p /\ theta m h' p' /\ p' lt' r)
